Update the Alloc pass
Renames the C -> locset calling convention to [cc_alloc], separate
typing constraints from the basic language interface, and use the new
framework to handle the RTL typing invariant.

backend/Conventions.v
@@ -142,92 +142,76 @@ Definition callee_save_loc (l: loc) :=
 Definition agree_callee_save (ls1 ls2: Locmap.t) : Prop :=
   forall l, callee_save_loc l -> ls1 l = ls2 l.
 
-Definition cc_locset: callconv li_c li_locset :=
+Inductive cc_alloc_mq: _ -> c_query -> locset_query -> Prop :=
+  cc_alloc_mq_intro id sg args rs m:
+    args = map (fun p => Locmap.getpair p rs) (loc_arguments sg) ->
+    cc_alloc_mq (sg, rs) (cq id sg args m) (lq id sg rs m).
+
+Inductive cc_alloc_mr: _ -> reply li_c -> reply li_locset -> Prop :=
+  cc_alloc_mr_intro sg rs res rs' m':
+    agree_callee_save rs rs' ->
+    Locmap.getpair (map_rpair R (loc_result sg)) rs' = res ->
+    cc_alloc_mr (sg, rs) (res, m') (rs', m').
+
+Definition cc_alloc: callconv li_c li_locset :=
   {|
-    world_def := unit;
+    ccworld := signature * Locmap.t;
     match_senv w := eq;
-    match_query_def w :=
-      fun '(cq id1 sg1 args m1) '(lq id2 sg2 rs m2) =>
-        id1 = id2 /\
-        sg1 = sg2 /\
-        args = map (fun p => Locmap.getpair p rs) (loc_arguments sg1) /\
-        m1 = m2 /\
-        (forall l, Val.has_type (rs l) (Loc.type l));
-    match_reply_def w :=
-      fun '(cq _ sg _ _) '(lq _ _ rs _) '(res, m1) '(rs', m2) =>
-        agree_callee_save rs rs' /\
-        Locmap.getpair (map_rpair R (loc_result sg)) rs' = res /\
-        m1 = m2;
+    match_query := cc_alloc_mq;
+    match_reply := cc_alloc_mr;
   |}.
 
-Notation ls_fb w := (cq_fb (world_q1 w)).
-Notation ls_sg w := (cq_sg (world_q1 w)).
-Notation ls_args w := (cq_args (world_q1 w)).
-Notation ls_rs w := (lq_rs (world_q2 w)).
-Notation ls_mem w := (cq_mem (world_q1 w)).
+Definition alloc_sg (w: ccworld cc_alloc) := fst w.
+Definition alloc_rs (w: ccworld cc_alloc) := snd w.
 
-Lemma match_cc_locset fb sg args rs m:
-  (forall l, Val.has_type (rs l) (Loc.type l)) ->
+Lemma match_cc_alloc fb sg args rs m:
   args = map (fun p => Locmap.getpair p rs) (loc_arguments sg) ->
   exists w,
-    match_query cc_locset w (cq fb sg args m) (lq fb sg rs m) /\
+    match_query cc_alloc w (cq fb sg args m) (lq fb sg rs m) /\
     forall vres m1' rs' m2',
-      match_reply cc_locset w (vres, m1') (rs', m2') ->
+      match_reply cc_alloc w (vres, m1') (rs', m2') ->
       agree_callee_save rs rs' /\
       Locmap.getpair (map_rpair R (loc_result sg)) rs' = vres /\
       m1' = m2'.
 Proof.
-  intros Hrs Hargs.
-  assert (Hq: match_query_def cc_locset tt (cq fb sg args m) (lq fb sg rs m)).
-  {
-    simpl; eauto.
-  }
-  eexists (mk_world _ _ _ _ Hq).
-  split. { constructor. }
-  intros vres m1' rs' m2' Hr.
-  inv Hr. simpl in *.
-  decompose [and] Hq3.
-  eauto.
+  intros Hargs.
+  exists (sg, rs). split.
+  - constructor; eauto.
+  - intros vres m1' rs' m2' Hr.
+    inv Hr. eauto.
 Qed.
 
-Lemma match_query_cc_locset (P: _->_->_->_->_->_->_-> Prop):
+Lemma match_query_cc_alloc (P: _ -> _ -> _ -> _ -> Prop):
   (forall id sg args rs m,
    args = map (fun p => Locmap.getpair p rs) (loc_arguments sg) ->
-   (forall l, Val.has_type (rs l) (Loc.type l)) ->
-   P id sg args rs m (cq id sg args m) (lq id sg rs m)) ->
-  (forall w q1 q2, match_query cc_locset w q1 q2 ->
-   P (ls_fb w) (ls_sg w) (ls_args w) (ls_rs w) (ls_mem w) q1 q2).
+   P sg rs (cq id sg args m) (lq id sg rs m)) ->
+  (forall w q1 q2, match_query cc_alloc w q1 q2 ->
+   P (alloc_sg w) (alloc_rs w) q1 q2).
 Proof.
   intros H w q1 q2 Hq.
-  destruct Hq as [w q1 q2 Hq].
-  destruct q1 as [id1 sg args m1], q2 as [id2 rs m2].
-  destruct Hq as (Hid & Hsg & Hargs & Hm & Hwt).
-  simpl in *; subst.
+  destruct Hq as [id sg args rs m]; simpl.
   eauto.
 Qed.
 
-Lemma match_reply_cc_locset w vres rs' m':
-  agree_callee_save (ls_rs w) rs' ->
-  Locmap.getpair (map_rpair R (loc_result (ls_sg w))) rs' = vres ->
-  match_reply cc_locset w (vres, m') (rs', m').
+Lemma match_reply_cc_alloc w vres rs' m':
+  agree_callee_save (snd w) rs' ->
+  Locmap.getpair (map_rpair R (loc_result (fst w))) rs' = vres ->
+  match_reply cc_alloc w (vres, m') (rs', m').
 Proof.
-  intros H.
-  destruct w as [w q1 q2 Hq].
-  destruct q1 as [id1 sg1 vargs m1], q2 as [id2 rs m2].
-  destruct Hq as (Hid & Hargs & Hm).
-  simpl in *.
-  constructor. split; eauto.
+  intros H Hvres.
+  destruct w as [sg rs].
+  constructor; eauto.
 Qed.
 
-Ltac inv_locset_query :=
+Ltac inv_alloc_query :=
   let w := fresh "w" in
   let q1 := fresh "q1" in
   let q2 := fresh "q2" in
   let Hq := fresh "Hq" in
   intros w q1 q2 Hq;
-  pattern (ls_fb w), (ls_sg w), (ls_args w), (ls_rs w), (ls_mem w), q1, q2;
+  pattern (alloc_sg w), (alloc_rs w), q1, q2;
   revert w q1 q2 Hq;
-  apply match_query_cc_locset.
+  apply match_query_cc_alloc.
 
 (* XXX may be needed later
 Lemma locmap_setpair_getpair p ls l:
